program_logic/OneToManyZK.ec
@@ -2,12 +2,12 @@ require import AllCore Distr FSet StdRing StdOrder StdBigop List.
 (*---*) import RField RealOrder Bigreal BRA.
 require import Aux.
 
-type prob, wit, sbits, event, auxiliary_input.
+type prob, wit, sbits, event.
 
 op E : event * sbits -> bool.
 
 require WhileCycle.
-clone import WhileCycle as MW with type irt    <- prob * auxiliary_input,
+clone import WhileCycle as MW with type irt    <- prob,
                                     type rrt   <- event * sbits,
                                     type sbits <- sbits,
                                     op MyPred <- E.
@@ -17,21 +17,21 @@ import MW.IFB.IM.
 
 
 module type Dist = {
-  proc guess(_:prob * wit * auxiliary_input * sbits) : bool
+  proc guess(_:prob * wit * sbits) : bool
 }.
 
 
 module type Simulator1 = {
-  proc run(Ny : prob, aux : auxiliary_input) : event * sbits
+  proc run(Ny : prob) : event * sbits
 }.
 
 
 module W0(Sim1:Simulator1,  D : Dist) = {
   module Sim1 = Sim1
-  proc run(a : prob, w : wit, aux : auxiliary_input) = {
+  proc run(a : prob, w : wit) = {
       var r, b;
-      r <@ Sim1.run(a,aux);
-      b <@ D.guess(a,w,aux,r.`2);
+      r <@ Sim1.run(a);
+      b <@ D.guess(a,w,r.`2);
       return (b, r);
   }
 }.
@@ -39,10 +39,10 @@ module W0(Sim1:Simulator1,  D : Dist) = {
 
 module W1(Sim1:Simulator1,  D : Dist) = {
   module M = W(Sim1)
-  proc run(a : (event * sbits -> bool) * (prob * auxiliary_input) * int * int * (event * sbits), w : wit) = {
+  proc run(a : (event * sbits -> bool) * (prob ) * int * int * (event * sbits), w : wit) = {
       var r, b;
       r <@ M.whp(a);
-      b <@ D.guess(a.`2.`1,w,a.`2.`2, r.`2);
+      b <@ D.guess(a.`2,w, r.`2);
       return (b, r);
   }
 }.
@@ -52,9 +52,9 @@ module W1(Sim1:Simulator1,  D : Dist) = {
 
 module Iter(Sim1 : Simulator1,  D : Dist)  = {
   module WI = W1(Sim1,D)
-  proc run(fevent : event, Ny : prob, w : wit, aux : auxiliary_input, ea : int, E : event * sbits -> bool) = {
+  proc run(fevent : event, Ny : prob, w : wit, ea : int, E : event * sbits -> bool) = {
     var r;
-    r <@ WI.run((E,(Ny,aux),1,ea,(fevent,witness)),w);
+    r <@ WI.run((E,(Ny),1,ea,(fevent,witness)),w);
     return r;
   }
 }.
@@ -104,42 +104,42 @@ apply oip3;auto.
 qed.
 
 
-local lemma zk_step2 &m E p ea w aux :
-  Pr[ W1(Sim1,D).run((E,(p,aux),1,ea,(fevent,witness)),w) 
+local lemma zk_step2 &m E p ea w  :
+  Pr[ W1(Sim1,D).run((E,(p),1,ea,(fevent,witness)),w) 
            @ &m : E res.`2 /\ res.`1 ]  
      = big predT
-        (fun i => Pr[W0(Sim1,D).run(p,w,aux) @ &m : !E res.`2] ^ i 
-         * Pr[ W0(Sim1,D).run(p,w,aux) @ &m : E res.`2 /\  res.`1] )
+        (fun i => Pr[W0(Sim1,D).run(p,w) @ &m : !E res.`2] ^ i 
+         * Pr[ W0(Sim1,D).run(p,w) @ &m : E res.`2 /\  res.`1] )
         (range 0 ea). 
 admitted.
 
 
-local lemma zk_step3 &m p eps ea coeff zkp (w : wit) aux:
-   `|Pr[ W0(Sim1,D).run(p,w,aux) @ &m : E res.`2 /\ res.`1]
-      / Pr[W0(Sim1,D).run(p,w,aux) @ &m : E res.`2] 
+local lemma zk_step3 &m p eps ea coeff zkp (w : wit):
+   `|Pr[ W0(Sim1,D).run(p,w) @ &m : E res.`2 /\ res.`1]
+      / Pr[W0(Sim1,D).run(p,w) @ &m : E res.`2] 
         - zkp| <= eps
-  => 0%r < Pr[W0(Sim1,D).run(p,w,aux) @ &m : E res.`2]  
+  => 0%r < Pr[W0(Sim1,D).run(p,w) @ &m : E res.`2]  
   => 0%r <= eps 
   => coeff = big predT
-               (fun i => Pr[W0(Sim1,D).run(p,w,aux) @ &m : !E res.`2] ^ i 
-                          * Pr[ W0(Sim1,D).run(p,w,aux) @ &m : E res.`2])
+               (fun i => Pr[W0(Sim1,D).run(p,w) @ &m : !E res.`2] ^ i 
+                          * Pr[ W0(Sim1,D).run(p,w) @ &m : E res.`2])
                (range 0 ea) 
   => exists (eps' : real), 
     0%r <= eps' <= eps   /\ 
-     `|Pr[ W1(Sim1,D).run((E,(p,aux),1,ea,(fevent,witness)), w   ) 
+     `|Pr[ W1(Sim1,D).run((E,(p),1,ea,(fevent,witness)), w   ) 
            @ &m : E res.`2 /\ res.`1 ]  
          - coeff * zkp| = coeff * eps'.
 proof. move => H0 H1 H2 coeffeq.
 have :  exists (eps' : real),  0%r <= eps' <= eps  
-  /\ `|Pr[ W0(Sim1,D).run(p,w,aux) @ &m : E res.`2 /\ res.`1] 
-         / Pr[W0(Sim1,D).run(p,w,aux) @ &m : E res.`2] 
+  /\ `|Pr[ W0(Sim1,D).run(p,w) @ &m : E res.`2 /\ res.`1] 
+         / Pr[W0(Sim1,D).run(p,w) @ &m : E res.`2] 
                 - zkp| = eps'
-  /\ (Pr[ W0(Sim1,D).run(p,w,aux) @ &m : E res.`2 /\ res.`1] 
-      = Pr[W0(Sim1,D).run(p,w,aux) @ &m : E res.`2]  
+  /\ (Pr[ W0(Sim1,D).run(p,w) @ &m : E res.`2 /\ res.`1] 
+      = Pr[W0(Sim1,D).run(p,w) @ &m : E res.`2]  
         * (zkp - eps')
       \/
-      Pr[ W0(Sim1,D).run(p,w,aux) @ &m : E res.`2 /\ res.`1] 
-      = Pr[W0(Sim1,D).run(p,w,aux) @ &m : E res.`2]  
+      Pr[ W0(Sim1,D).run(p,w) @ &m : E res.`2 /\ res.`1] 
+      = Pr[W0(Sim1,D).run(p,w) @ &m : E res.`2]  
         * (zkp + eps')).
 apply (zk_step1 &m). assumption. assumption. assumption.
 elim. move => eps' [H3 [H41 H42 ]].
@@ -147,31 +147,31 @@ exists eps'.
 split. auto.
 apply oip4.
 rewrite coeffeq.
-have ->: Pr[W0(Sim1,D).run(p,w,aux) @ &m : ! E res.`2]
-  = 1%r - Pr[W0(Sim1,D).run(p,w,aux) @ &m :  E res.`2].
-  have ->: 1%r = Pr[W0(Sim1,D).run(p,w,aux) @ &m :  true].
+have ->: Pr[W0(Sim1,D).run(p,w) @ &m : ! E res.`2]
+  = 1%r - Pr[W0(Sim1,D).run(p,w) @ &m :  E res.`2].
+  have ->: 1%r = Pr[W0(Sim1,D).run(p,w) @ &m :  true].
   byphoare. 
 proc. call D_ll. call Sim1_ll.  auto. auto. auto.
-  have ->: Pr[W0(Sim1,D).run(p,w,aux) @ &m : true] = Pr[W0(Sim1,D).run(p,w,aux) @ &m : E res.`2]
-   + Pr[W0(Sim1,D).run(p,w,aux) @ &m : !E res.`2]. rewrite Pr[mu_split E res.`2]. 
+  have ->: Pr[W0(Sim1,D).run(p,w) @ &m : true] = Pr[W0(Sim1,D).run(p,w) @ &m : E res.`2]
+   + Pr[W0(Sim1,D).run(p,w) @ &m : !E res.`2]. rewrite Pr[mu_split E res.`2]. 
   simplify. smt. smt.
   have : 0%r <=
 bigi predT
   (fun (i : int) =>
-     (1%r - Pr[W0(Sim1,D).run(p,w,aux) @ &m : E res.`2]) ^ i *
-     Pr[W0(Sim1,D).run(p,w,aux) @ &m : E res.`2]) 0 ea.
-  apply (big_geq0  Pr[W0(Sim1,D).run(p,w,aux) @ &m : E res.`2] _ ea). smt.
+     (1%r - Pr[W0(Sim1,D).run(p,w) @ &m : E res.`2]) ^ i *
+     Pr[W0(Sim1,D).run(p,w) @ &m : E res.`2]) 0 ea.
+  apply (big_geq0  Pr[W0(Sim1,D).run(p,w) @ &m : E res.`2] _ ea). smt.
   smt. 
-case (Pr[ W0(Sim1,D).run(p,w,aux) @ &m : E res.`2 /\ res.`1] 
-      = Pr[W0(Sim1,D).run(p,w,aux) @ &m : E res.`2]  
+case (Pr[ W0(Sim1,D).run(p,w) @ &m : E res.`2 /\ res.`1] 
+      = Pr[W0(Sim1,D).run(p,w) @ &m : E res.`2]  
         * (zkp + eps')).
 progress. rewrite /(\o).
 rewrite zk_step2. 
 rewrite H. simplify.
 have : bigi predT
   (fun (i : int) =>
-     Pr[W0(Sim1,D).run(p,w,aux) @ &m : ! E res.`2] ^ i *
-     (Pr[W0(Sim1,D).run(p,w,aux) @ &m : E res.`2] *
+     Pr[W0(Sim1,D).run(p,w) @ &m : ! E res.`2] ^ i *
+     (Pr[W0(Sim1,D).run(p,w) @ &m : E res.`2] *
       (zkp + eps'))) 0 ea =
 coeff * zkp + coeff * eps'.
 rewrite coeffeq.
@@ -181,8 +181,8 @@ rewrite - big_split.
 simplify. smt.
 timeout 20. smt.
 move => H5.
-have : Pr[ W0(Sim1,D).run(p,w,aux) @ &m : E res.`2 /\ res.`1] 
-        = Pr[W0(Sim1,D).run(p,w,aux) @ &m : E res.`2]  
+have : Pr[ W0(Sim1,D).run(p,w) @ &m : E res.`2 /\ res.`1] 
+        = Pr[W0(Sim1,D).run(p,w) @ &m : E res.`2]  
           * (zkp - eps').
 smt.
 progress. rewrite /(\o).
@@ -190,8 +190,8 @@ rewrite zk_step2.
 rewrite H. simplify.
 have : bigi predT
   (fun (i : int) =>
-     Pr[W0(Sim1,D).run(p,w,aux) @ &m : ! E res.`2] ^ i *
-     (Pr[W0(Sim1,D).run(p,w,aux) @ &m : E res.`2] *
+     Pr[W0(Sim1,D).run(p,w) @ &m : ! E res.`2] ^ i *
+     (Pr[W0(Sim1,D).run(p,w) @ &m : E res.`2] *
       (zkp - eps'))) 0 ea =
 coeff * zkp - coeff * eps'.
 rewrite coeffeq.
@@ -203,43 +203,43 @@ timeout 20. smt.
 qed.
 
 
-local lemma zk_non_final &m p  eps ea coeff zkp w aux:
-   `|Pr[ W0(Sim1,D).run(p,w,aux) @ &m : E res.`2 /\  res.`1] 
-          / Pr[W0(Sim1,D).run(p,w,aux) @ &m : E res.`2 ] 
+local lemma zk_non_final &m p  eps ea coeff zkp w :
+   `|Pr[ W0(Sim1,D).run(p,w) @ &m : E res.`2 /\  res.`1] 
+          / Pr[W0(Sim1,D).run(p,w) @ &m : E res.`2 ] 
         - zkp| <= eps
-  => 0%r < Pr[W0(Sim1,D).run(p,w,aux) @ &m : E res.`2] 
+  => 0%r < Pr[W0(Sim1,D).run(p,w) @ &m : E res.`2] 
   => 0%r <= eps                 (* not needed *)
   => coeff = big predT
-               (fun i => Pr[W0(Sim1,D).run(p,w,aux) @ &m : !E res.`2] ^ i 
-                          * Pr[ W0(Sim1,D).run(p,w,aux) @ &m : E res.`2])
+               (fun i => Pr[W0(Sim1,D).run(p,w) @ &m : !E res.`2] ^ i 
+                          * Pr[ W0(Sim1,D).run(p,w) @ &m : E res.`2])
                (range 0 ea) 
-  => `|Pr[ Iter(Sim1, D).run((fevent, p, w,aux,ea,E) ) 
+  => `|Pr[ Iter(Sim1, D).run((fevent, p, w,ea,E) ) 
            @ &m : E res.`2 /\ res.`1 ]  
               - coeff * zkp| <= eps.
 proof. move => H1 H2 H3 H4. 
 have ->: 
-  Pr[Iter(Sim1, D).run(fevent, p, w, aux,ea, E) @ &m :
+  Pr[Iter(Sim1, D).run(fevent, p, w, ea, E) @ &m :
      E res.`2 /\ res.`1]
-  = Pr[ W1(Sim1,D).run((E,(p,aux),1,ea,(fevent,witness)), w) 
+  = Pr[ W1(Sim1,D).run((E,(p),1,ea,(fevent,witness)), w) 
            @ &m : E res.`2 /\ res.`1 ] .  
  byequiv (_: _==> ={res}). proc*.
 inline Iter(Sim1, D).run. sp. wp. 
 inline W1(Sim1, D).run. sp. 
 seq 1 1 :   (a0{2} = a{2} /\
   w0{2} = w{2} /\
-  a{1} = (E0{1}, (Ny0{1}, aux0{1}), 1, ea0{1}, (fevent0{1}, witness)) /\
+  a{1} = (E0{1}, (Ny0{1}), 1, ea0{1}, (fevent0{1}, witness)) /\
   w1{1} = w0{1} /\
   fevent0{1} = fevent{1} /\
   Ny0{1} = Ny{1} /\
   w0{1} = w{1} /\
-  aux0{1} = aux{1} /\
+
   ea0{1} = ea{1} /\
   E0{1} = E{1} /\
-  (a{2}, w{2}) = ((Top.E, (p, aux), 1, ea, (Top.fevent, witness)), w) /\
+  (a{2}, w{2}) = ((Top.E, (p), 1, ea, (Top.fevent, witness)), w) /\
   (glob D){2} = (glob D){m} /\
   (glob Sim1){2} = (glob Sim1){m} /\
-  (fevent{1}, Ny{1}, w{1}, aux{1}, ea{1}, E{1}) =
-  (Top.fevent, p, w, aux, ea, Top.E) /\
+  (fevent{1}, Ny{1}, w{1},  ea{1}, E{1}) =
+  (Top.fevent, p, w,  ea, Top.E) /\
   (glob D){1} = (glob D){m} /\ (glob Sim1){1} = (glob Sim1){m} /\ r1{1} = r0{2}).
 admit. wp. call (_:true). skip. progress. smt. auto. auto.
 
@@ -250,22 +250,22 @@ admit. wp. call (_:true). skip. progress. smt. auto. auto.
 (* skip. smt. auto. auto. *)
 have : coeff <= 1%r. 
 rewrite H4.
-have ->: Pr[W0(Sim1,D).run(p,w,aux) @ &m : ! E res.`2]
-  = 1%r - Pr[W0(Sim1,D).run(p,w,aux) @ &m :  E res.`2].
-  have ->: 1%r = Pr[W0(Sim1,D).run(p,w,aux) @ &m :  true].
+have ->: Pr[W0(Sim1,D).run(p,w) @ &m : ! E res.`2]
+  = 1%r - Pr[W0(Sim1,D).run(p,w) @ &m :  E res.`2].
+  have ->: 1%r = Pr[W0(Sim1,D).run(p,w) @ &m :  true].
   byphoare. proc.  call D_ll. call Sim1_ll. auto. auto. auto.
-  have ->: Pr[W0(Sim1,D).run(p,w,aux) @ &m : true] = Pr[W0(Sim1,D).run(p,w,aux) @ &m : E res.`2]
-   + Pr[W0(Sim1,D).run(p,w,aux) @ &m : !E res.`2]. rewrite Pr[mu_split E res.`2]. 
+  have ->: Pr[W0(Sim1,D).run(p,w) @ &m : true] = Pr[W0(Sim1,D).run(p,w) @ &m : E res.`2]
+   + Pr[W0(Sim1,D).run(p,w) @ &m : !E res.`2]. rewrite Pr[mu_split E res.`2]. 
   simplify. smt. smt.
   have : 
 bigi predT
   (fun (i : int) =>
-     (1%r - Pr[W0(Sim1,D).run(p,w,aux) @ &m : E res.`2]) ^ i *
-     Pr[W0(Sim1,D).run(p,w,aux) @ &m : E res.`2]) 0 ea <= 1%r.
-  apply (big_leq1  Pr[W0(Sim1,D).run(p,w,aux) @ &m : E res.`2] _ ea). smt.
+     (1%r - Pr[W0(Sim1,D).run(p,w) @ &m : E res.`2]) ^ i *
+     Pr[W0(Sim1,D).run(p,w) @ &m : E res.`2]) 0 ea <= 1%r.
+  apply (big_leq1  Pr[W0(Sim1,D).run(p,w) @ &m : E res.`2] _ ea). smt.
   smt.
 move => H6.
-have : exists eps', 0%r <= eps' <= eps /\ `|Pr[W1(Sim1,D).run((E, (p,aux), 1, ea,
+have : exists eps', 0%r <= eps' <= eps /\ `|Pr[W1(Sim1,D).run((E, (p), 1, ea,
                  (fevent, witness)),w) @ &m :
      E res.`2 /\ res.`1] -
   coeff * zkp| 
@@ -280,21 +280,21 @@ smt.
 qed.
 
 
-local lemma zk_almost_final &m p w eps ea coeff zkp aux:
-   `|Pr[ W0(Sim1,D).run(p,w,aux) @ &m : E res.`2 /\ res.`1] 
-        / Pr[W0(Sim1,D).run(p,w,aux) @ &m : E res.`2] 
+local lemma zk_almost_final &m p w eps ea coeff zkp :
+   `|Pr[ W0(Sim1,D).run(p,w) @ &m : E res.`2 /\ res.`1] 
+        / Pr[W0(Sim1,D).run(p,w) @ &m : E res.`2] 
         - zkp| <= eps
-  => 0%r < Pr[W0(Sim1,D).run(p,w,aux) @ &m : E res.`2] 
+  => 0%r < Pr[W0(Sim1,D).run(p,w) @ &m : E res.`2] 
   => coeff = big predT
-               (fun i => Pr[W0(Sim1,D).run(p,w,aux) @ &m : !E res.`2] ^ i 
-                         * Pr[ W0(Sim1,D).run(p,w,aux) @ &m : E res.`2])
+               (fun i => Pr[W0(Sim1,D).run(p,w) @ &m : !E res.`2] ^ i 
+                         * Pr[ W0(Sim1,D).run(p,w) @ &m : E res.`2])
                (range 0 ea) 
-  => `|Pr[ Iter(Sim1, D).run((fevent, p,w,aux,ea,E)) 
+  => `|Pr[ Iter(Sim1, D).run((fevent, p,w,ea,E)) 
            @ &m : E res.`2 /\ res.`1 ]  
          - zkp| <= eps + (1%r - coeff).
 proof.
 move => H1 H2 H3.
-have ie1 : `|Pr[ Iter(Sim1, D).run(fevent, p,w,aux,ea,E) 
+have ie1 : `|Pr[ Iter(Sim1, D).run(fevent, p,w,ea,E) 
            @ &m : E res.`2 /\  res.`1 ]  
          - coeff * zkp| <= eps.
 apply (zk_non_final &m p eps ea coeff zkp);auto. smt.
@@ -303,137 +303,137 @@ auto.
 qed.
 
 
-local lemma zk_final &m p w eps ea zkp aux:
-   `|Pr[ W0(Sim1,D).run(p,w,aux) @ &m : E res.`2 /\ res.`1] 
-        / Pr[W0(Sim1,D).run(p,w,aux) @ &m : E res.`2] 
+local lemma zk_final &m p w eps ea zkp:
+   `|Pr[ W0(Sim1,D).run(p,w) @ &m : E res.`2 /\ res.`1] 
+        / Pr[W0(Sim1,D).run(p,w) @ &m : E res.`2] 
         - zkp| <= eps
   => 0 <= ea
-  => `|Pr[ Iter(Sim1, D).run(fevent,p,w,aux,ea,E) 
+  => `|Pr[ Iter(Sim1, D).run(fevent,p,w,ea,E) 
            @ &m : E res.`2 /\ res.`1 ]  
          - zkp| 
-           <= eps + Pr[W0(Sim1,D).run(p,w,aux) @ &m : !E res.`2] ^ ea.
+           <= eps + Pr[W0(Sim1,D).run(p,w) @ &m : !E res.`2] ^ ea.
 proof. 
-case (0%r = Pr[W0(Sim1,D).run(p,w,aux) @ &m : E res.`2]).
+case (0%r = Pr[W0(Sim1,D).run(p,w) @ &m : E res.`2]).
 move => r. rewrite - r. simplify. progress.
-have <-: 1%r = Pr[W0(Sim1,D).run(p,w,aux) @ &m : ! E res.`2]. 
-  have ->: 1%r = Pr[W0(Sim1,D).run(p,w,aux) @ &m : true ].  
+have <-: 1%r = Pr[W0(Sim1,D).run(p,w) @ &m : ! E res.`2]. 
+  have ->: 1%r = Pr[W0(Sim1,D).run(p,w) @ &m : true ].  
   byphoare. proc. call D_ll. call Sim1_ll. auto. auto. auto.
   rewrite Pr[mu_split (E res.`2)]. simplify. rewrite - r. 
   simplify. auto.
 have ->: 1%r ^ ea = 1%r. smt.
 smt.
 progress.
-have f : 0%r < Pr[W0(Sim1,D).run(p,w,aux) @ &m : E res.`2].  smt.
-have ->: Pr[W0(Sim1,D).run(p,w,aux) @ &m : !E res.`2] ^ ea
- = 1%r - (1%r - Pr[W0(Sim1,D).run(p,w,aux) @ &m : !E res.`2] ^ ea).
+have f : 0%r < Pr[W0(Sim1,D).run(p,w) @ &m : E res.`2].  smt.
+have ->: Pr[W0(Sim1,D).run(p,w) @ &m : !E res.`2] ^ ea
+ = 1%r - (1%r - Pr[W0(Sim1,D).run(p,w) @ &m : !E res.`2] ^ ea).
 smt.
 rewrite - big_formula_p. smt. auto. progress.
-have ->: (1%r - Pr[W0(Sim1,D).run(p,w,aux) @ &m : ! E res.`2])
- = Pr[W0(Sim1,D).run(p,w,aux) @ &m : E res.`2].
-have ->: 1%r = Pr[W0(Sim1,D).run(p,w,aux) @ &m :  true].
+have ->: (1%r - Pr[W0(Sim1,D).run(p,w) @ &m : ! E res.`2])
+ = Pr[W0(Sim1,D).run(p,w) @ &m : E res.`2].
+have ->: 1%r = Pr[W0(Sim1,D).run(p,w) @ &m :  true].
 byphoare.
 proc.  call D_ll. call Sim1_ll. auto. auto. auto.
-have ->: Pr[W0(Sim1,D).run(p,w,aux) @ &m : true] = Pr[W0(Sim1,D).run(p,w,aux) @ &m : ! E res.`2]
- + Pr[W0(Sim1,D).run(p,w,aux) @ &m : E res.`2]. rewrite Pr[mu_split ! E res.`2].
+have ->: Pr[W0(Sim1,D).run(p,w) @ &m : true] = Pr[W0(Sim1,D).run(p,w) @ &m : ! E res.`2]
+ + Pr[W0(Sim1,D).run(p,w) @ &m : E res.`2]. rewrite Pr[mu_split ! E res.`2].
 simplify. smt. smt.
 apply (zk_almost_final &m);auto.
 qed.
 
 
-local lemma zk_final_le &m p w p0 eps ea zkp aux:
-   `|Pr[ W0(Sim1,D).run(p,w,aux) @ &m : E res.`2 /\ res.`1] 
-        / Pr[W0(Sim1,D).run(p,w,aux) @ &m : E res.`2] - zkp| <= eps
+local lemma zk_final_le &m p w p0 eps ea zkp:
+   `|Pr[ W0(Sim1,D).run(p,w) @ &m : E res.`2 /\ res.`1] 
+        / Pr[W0(Sim1,D).run(p,w) @ &m : E res.`2] - zkp| <= eps
   => 0 <= ea
-  => Pr[W0(Sim1,D).run(p,w,aux) @ &m : E res.`2] >= p0
-  => `|Pr[ Iter(Sim1, D).run(fevent,p,w,aux,ea,E) 
+  => Pr[W0(Sim1,D).run(p,w) @ &m : E res.`2] >= p0
+  => `|Pr[ Iter(Sim1, D).run(fevent,p,w,ea,E) 
            @ &m : E res.`2 /\ res.`1 ] - zkp| 
               <= eps + (1%r-p0) ^ ea.
 progress.
 have fff : p0 <= 1%r. smt.
-have f1 : `|Pr[ Iter(Sim1, D).run(fevent, p,w,aux,ea,E) 
+have f1 : `|Pr[ Iter(Sim1, D).run(fevent, p,w,ea,E) 
            @ &m : E res.`2 /\ res.`1 ]  
          - zkp| 
-      <= eps + (1%r - Pr[W0(Sim1,D).run(p,w,aux) @ &m : E res.`2] )^ea.
-have ->: (1%r - Pr[W0(Sim1,D).run(p,w,aux) @ &m : E res.`2] ) = 
-  (Pr[W0(Sim1,D).run(p,w,aux) @ &m : !E res.`2] ). 
-have ->: 1%r = Pr[W0(Sim1,D).run(p,w,aux) @ &m :  true].
+      <= eps + (1%r - Pr[W0(Sim1,D).run(p,w) @ &m : E res.`2] )^ea.
+have ->: (1%r - Pr[W0(Sim1,D).run(p,w) @ &m : E res.`2] ) = 
+  (Pr[W0(Sim1,D).run(p,w) @ &m : !E res.`2] ). 
+have ->: 1%r = Pr[W0(Sim1,D).run(p,w) @ &m :  true].
 byphoare. proc. call D_ll. call Sim1_ll. auto. auto. auto.
-have ->: Pr[W0(Sim1,D).run(p,w,aux) @ &m : true] = Pr[W0(Sim1,D).run(p,w,aux) @ &m : ! E res.`2]
- + Pr[W0(Sim1,D).run(p,w,aux) @ &m : E res.`2]. rewrite Pr[mu_split ! E res.`2]. 
+have ->: Pr[W0(Sim1,D).run(p,w) @ &m : true] = Pr[W0(Sim1,D).run(p,w) @ &m : ! E res.`2]
+ + Pr[W0(Sim1,D).run(p,w) @ &m : E res.`2]. rewrite Pr[mu_split ! E res.`2]. 
 simplify. smt. smt.
 apply (zk_final &m).
 have f2 : 
- (1%r - Pr[W0(Sim1,D).run(p,w,aux) @ &m : E res.`2]) <= (1%r - p0). smt.
-have f3 : (1%r - Pr[W0(Sim1,D).run(p,w,aux) @ &m : E res.`2]) ^ ea <= (1%r - p0) ^ ea.
+ (1%r - Pr[W0(Sim1,D).run(p,w) @ &m : E res.`2]) <= (1%r - p0). smt.
+have f3 : (1%r - Pr[W0(Sim1,D).run(p,w) @ &m : E res.`2]) ^ ea <= (1%r - p0) ^ ea.
 apply multn2;auto. smt. auto. auto. auto. smt.
 qed.
 
 
-local lemma zk_final_clean' &m p w p0 eps ea zkp aux:
-     `| Pr[ W0(Sim1,D).run(p,w,aux) @ &m : E res.`2 /\ res.`1 ]
-           / Pr[W0(Sim1,D).run(p,w,aux) @ &m : E res.`2 ] - zkp | <= eps
+local lemma zk_final_clean' &m p w p0 eps ea zkp:
+     `| Pr[ W0(Sim1,D).run(p,w) @ &m : E res.`2 /\ res.`1 ]
+           / Pr[W0(Sim1,D).run(p,w) @ &m : E res.`2 ] - zkp | <= eps
   => 0  <= ea
-  => p0 <= Pr[W0(Sim1,D).run(p,w,aux) @ &m : E res.`2 ]
-  => `| Pr[Iter(Sim1, D).run(fevent,p,w,aux,ea,E) @ &m : res.`1] - zkp |
+  => p0 <= Pr[W0(Sim1,D).run(p,w) @ &m : E res.`2 ]
+  => `| Pr[Iter(Sim1, D).run(fevent,p,w,ea,E) @ &m : res.`1] - zkp |
               <= eps + 2%r * (1%r-p0) ^ ea.
 proof. progress.
-have bf :  `|Pr[ Iter(Sim1, D).run(fevent,p,w,aux,ea,E) 
+have bf :  `|Pr[ Iter(Sim1, D).run(fevent,p,w,ea,E) 
            @ &m : res.`1 ] - zkp| 
               <= (eps + (1%r-p0) ^ ea ) +
-(Pr[ Iter(Sim1, D).run(fevent,p,w,aux,ea,E) 
+(Pr[ Iter(Sim1, D).run(fevent,p,w,ea,E) 
            @ &m : !E res.`2]).
-have f1 : `|Pr[ Iter(Sim1, D).run(fevent,p,w,aux,ea,E) 
+have f1 : `|Pr[ Iter(Sim1, D).run(fevent,p,w,ea,E) 
            @ &m : E res.`2 /\ res.`1 ] - zkp| 
               <= eps + (1%r-p0) ^ ea.
-apply (zk_final_le &m p w p0 eps ea zkp aux);auto.
-apply (kkk Pr[Iter(Sim1, D).run(fevent, p, w, aux, ea, E) @ &m : res.`1]
-Pr[Iter(Sim1, D).run(fevent, p, w, aux, ea, E) @ &m :
+apply (zk_final_le &m p w p0 eps ea zkp );auto.
+apply (kkk Pr[Iter(Sim1, D).run(fevent, p, w,  ea, E) @ &m : res.`1]
+Pr[Iter(Sim1, D).run(fevent, p, w,  ea, E) @ &m :
          E res.`2 /\ res.`1]). smt.
 rewrite Pr[mu_split E res.`2] .
-have ->: Pr[Iter(Sim1, D).run(fevent, p, w, aux, ea, E) @ &m : res.`1 /\ E res.`2]
- = Pr[Iter(Sim1, D).run(fevent, p, w, aux, ea, E) @ &m : E res.`2 /\ res.`1 ].
+have ->: Pr[Iter(Sim1, D).run(fevent, p, w, ea, E) @ &m : res.`1 /\ E res.`2]
+ = Pr[Iter(Sim1, D).run(fevent, p, w, ea, E) @ &m : E res.`2 /\ res.`1 ].
 smt.
 smt.
 auto.  
 clear H.
-have bf2 : Pr[Iter(Sim1, D).run(fevent, p, w, aux, ea, E) @ &m : ! E res.`2]
+have bf2 : Pr[Iter(Sim1, D).run(fevent, p, w, ea, E) @ &m : ! E res.`2]
   <= (1%r - p0) ^ ea.
-  have bf3: Pr[W0(Sim1, D).run(p, w, aux) @ &m : !E res.`2] <= 1%r - p0.
-    have -> : 1%r = Pr[W0(Sim1, D).run(p, w, aux) @ &m : true]. byphoare.
+  have bf3: Pr[W0(Sim1, D).run(p, w) @ &m : !E res.`2] <= 1%r - p0.
+    have -> : 1%r = Pr[W0(Sim1, D).run(p, w) @ &m : true]. byphoare.
     proc. call D_ll. call Sim1_ll. auto. auto. auto.
-       have : Pr[W0(Sim1, D).run(p, w, aux) @ &m : true] 
-                - Pr[W0(Sim1, D).run(p, w, aux) @ &m : !E res.`2] 
-                 = Pr[W0(Sim1, D).run(p, w, aux) @ &m : E res.`2]. 
+       have : Pr[W0(Sim1, D).run(p, w) @ &m : true] 
+                - Pr[W0(Sim1, D).run(p, w) @ &m : !E res.`2] 
+                 = Pr[W0(Sim1, D).run(p, w) @ &m : E res.`2]. 
     rewrite Pr[mu_split E res.`2]. simplify. smt. smt. 
 
-  have ->: Pr[Iter(Sim1, D).run(fevent, p, w, aux, ea, E) @ &m : ! E res.`2] 
-     = Pr[ W(Sim1).whp(E,(p,aux),1,ea,(fevent,witness)) @ &m : ! E res ].
+  have ->: Pr[Iter(Sim1, D).run(fevent, p, w, ea, E) @ &m : ! E res.`2] 
+     = Pr[ W(Sim1).whp(E,(p),1,ea,(fevent,witness)) @ &m : ! E res ].
    byequiv. proc*.  inline Iter(Sim1, D).run. sp. wp. inline Iter(Sim1, D).WI.run.
  sp. wp. call {1} D_ll. 
   conseq (_: _==> r1{1} = r0{2}). smt.
 call (_: ={glob Sim1}).  sim. skip. progress. auto. auto.
 apply (final_zz_le (Sim1) Sim1_ll _ &m). apply Sim1_rew_ph. smt. auto. 
-have ->: Pr[Sim1.run(p,aux) @ &m : ! E res] 
-  = Pr[W0(Sim1, D).run(p, w, aux) @ &m : ! E res.`2].
+have ->: Pr[Sim1.run(p) @ &m : ! E res] 
+  = Pr[W0(Sim1, D).run(p, w) @ &m : ! E res.`2].
 byequiv. proc*. inline*. wp. sp. call {2} D_ll. call (_: true).
   skip. progress. auto. auto. auto.
 smt. auto. auto. auto. smt.
 qed.
 
 
-lemma one_to_many_zk &m p w p0 eps ea zkp aux:
-     `| Pr[ W0(Sim1,D).run(p,w,aux) @ &m : E res.`2 /\ res.`1 ]
-           / Pr[Sim1.run(p,aux) @ &m : E res]  - zkp | <= eps
+lemma one_to_many_zk &m p w p0 eps ea zkp:
+     `| Pr[ W0(Sim1,D).run(p,w) @ &m : E res.`2 /\ res.`1 ]
+           / Pr[Sim1.run(p) @ &m : E res]  - zkp | <= eps
   => 0  <= ea
-  => p0 <= Pr[Sim1.run(p,aux) @ &m :  E res] 
-  => `| Pr[Iter(Sim1, D).run(fevent,p,w,aux,ea,E) @ &m : res.`1] - zkp |
+  => p0 <= Pr[Sim1.run(p) @ &m :  E res] 
+  => `| Pr[Iter(Sim1, D).run(fevent,p,w,ea,E) @ &m : res.`1] - zkp |
               <= eps + 2%r * (1%r-p0) ^ ea.
-have ->: Pr[Sim1.run(p,aux) @ &m : E res] 
-  = Pr[W0(Sim1, D).run(p, w, aux) @ &m :  E res.`2].
+have ->: Pr[Sim1.run(p) @ &m : E res] 
+  = Pr[W0(Sim1, D).run(p, w) @ &m :  E res.`2].
 byequiv. proc*. inline*. wp. sp. call {2} D_ll. call (_: true).
   skip. progress. auto. auto. auto.
 progress.
-smt. auto.  auto. apply (zk_final_clean' &m p w p0 eps ea zkp aux);auto.
+smt. auto.  auto. apply (zk_final_clean' &m p w p0 eps ea zkp);auto.
 qed.
 end section.
 
