QR/Soundness.ec
@@ -8,16 +8,16 @@ section.
 declare module P <: MaliciousProver {-HonestVerifier}.
 declare axiom P_response_ll : islossless P.response.
 
-local lemma qr_soundness_ph s ax :
+local lemma qr_soundness_ph s  :
    ! in_language IsSqRoot s => 
-   phoare [ Soundness(P,HonestVerifier).run : arg = (s,ax) ==> res ] <= (1%r/2%r).
+   phoare [ Soundness(P,HonestVerifier).run : arg = (s) ==> res ] <= (1%r/2%r).
 proof. move => qra.
 proc. inline*. 
 wp.
-seq 3 : ((statement,aux) = (s,ax) /\ statement0 = statement /\ commitment = commit) (1%r) (1%r/2%r) (0%r) (1%r).  auto. auto.
+seq 3 : ((statement) = (s) /\ statement0 = statement /\ commitment = commit) (1%r) (1%r/2%r) (0%r) (1%r).  auto. auto.
 exists* commit. elim*. move => cv.
 case (!IsQR cv).
-seq 1 : (!challenge0) (1%r/2%r) (0%r) (1%r/2%r) (1%r) (cv = commit /\ s = statement /\ ax = aux /\ !IsQR cv).
+seq 1 : (!challenge0) (1%r/2%r) (0%r) (1%r/2%r) (1%r) (cv = commit /\ s = statement  /\ !IsQR cv).
 rnd.  skip. auto.
 hoare. call (_:true ==> true). auto.
 wp. auto. progress. rewrite H0. simplify.   timeout 20. smt. 
@@ -27,7 +27,7 @@ have ->: mu1 (duniform [false; true]) true = 1%r/2%r.
 rewrite duniform1E_uniq. auto. simplify. auto. auto.
 simplify. 
 conseq (_: _ ==> true). call (_: true ==> true). auto.  auto. auto.
-seq 1 : (!challenge0) (1%r/2%r) (0%r) (1%r/2%r) (1%r) (cv = commit /\ s = statement /\ ax = aux /\ IsQR cv).
+seq 1 : (!challenge0) (1%r/2%r) (0%r) (1%r/2%r) (1%r) (cv = commit /\ s = statement  /\ IsQR cv).
 rnd. skip. auto.
 hoare. 
 call (_:true ==> true). auto.  
@@ -43,12 +43,12 @@ simplify. auto. call (_ : true ==> true).  auto. skip. auto. auto.
 qed.
 
 
-lemma qr_soundness &m s ax:
+lemma qr_soundness &m s:
     ! in_language IsSqRoot s =>
-     Pr[Soundness(P, HonestVerifier).run(s, ax) @ &m : res]
+     Pr[Soundness(P, HonestVerifier).run(s) @ &m : res]
      <= 1%r/2%r.
-progress. byphoare (_: arg = (s,ax) ==> _);auto.
-apply (qr_soundness_ph s ax);auto.
+progress. byphoare (_: arg = (s) ==> _);auto.
+apply (qr_soundness_ph s);auto.
 qed.
 
 
